rupicola/SemanticTyping.fst
@@ -31,35 +31,13 @@ let lem_value_is_typed_exp e t
   : Lemma (e ∈ t ==> e ⋮ t)
   = admit () (** Amal uses such a lemma **)
 
-(** ground substitution / value environment **)
-let gsub (g:env) (b:bool{b ==> (forall x. None? (g x))}) = (** CA: this b is polluting **)
-  s:(sub b){forall x. Some? (g x) ==> is_value (s x) /\ (s x) ∈ (Some?.v (g x))}
-
-let gsub_empty : gsub empty true =
-  (fun v -> EVar v)
-
-let gsub_extend (#g:env) #b (s:gsub g b) (t:typ) (v:value{v ∈ t}) : gsub (extend t g) false =
-  let f = fun (y:var) -> if y = 0 then v else s (y-1) in
-  introduce exists (x:var). ~(EVar? (f x)) with 0 and ();
-  f
-
-let gsubst (#g:env) #b (s:gsub g b) (e:exp{fv_in_env g e}) : closed_exp =
-  lem_subst_freevars_closes_exp s e 0;
-  subst s e
-
-let lem_substitution #g #b (s:gsub g b) (t:typ) (v:value{v ∈ t}) (e:exp)
-  : Lemma (
-    (subst (sub_beta v) (subst (sub_elam s) e)) == (subst (gsub_extend s t v) e))
-  = admit () (** common lemma **)
-
-let lem_gsubst_empty_identity (e:closed_exp) :
-  Lemma (gsubst gsub_empty e == e)
-  [SMTPat (gsubst gsub_empty e)] =
-  admit ()
+let gsub_only_values #g #b (s:gsub g b) =
+  forall x. Some? (g x) ==> (s x) ∈ (Some?.v (g x))
 
 let sem_typing (g:env) (e:exp) (t:typ) : Type0 =
   fv_in_env g e /\
-  (forall b (s:gsub g b). (gsubst s e) ⋮ t)
+  (forall b (s:gsub g b).
+    gsub_only_values s ==>  (gsubst s e) ⋮ t)
 
 let lem_sem_typing_closed (e:exp) (t:typ) :
   Lemma (requires sem_typing empty e t)
@@ -102,22 +80,23 @@ let typing_rule_lam g (t1:typ) (body:exp) (t2:typ) : Lemma
   let g' = extend t1 g in
   assert (fv_in_env g' body);
   assume (fv_in_env g (ELam body));
-  introduce forall b (s:gsub g b). gsubst s (ELam body) ⋮ TArr t1 t2 with begin
-    let g' = extend t1 g in
-    let body' = subst (sub_elam s) body in
-    assert (gsubst s (ELam body) == ELam body');
-    introduce forall (v:value). v ∈ t1 ==>  subst_beta v body' ⋮ t2 with begin
-      introduce _ ==> _ with _. begin
-        assert (sem_typing g' body t2);
-        eliminate forall b (s:gsub g' b). (gsubst s body) ⋮ t2 with false (gsub_extend s t1 v);
-        assert (gsubst (gsub_extend s t1 v) body ⋮ t2);
-        lem_substitution s t1 v body;
-        assert (subst_beta v body' ⋮ t2)
-      end
-    end;
-    assert (gsubst s (ELam body) ∈ TArr t1 t2);
-    lem_value_is_typed_exp (gsubst s (ELam body)) (TArr t1 t2)
-  end
+  introduce forall b (s:gsub g b). gsub_only_values s ==> gsubst s (ELam body) ⋮ TArr t1 t2 with
+    introduce _ ==> _ with _. begin
+      let g' = extend t1 g in
+      let body' = subst (sub_elam s) body in
+      assert (gsubst s (ELam body) == ELam body');
+      introduce forall (v:value). v ∈ t1 ==>  subst_beta v body' ⋮ t2 with begin
+        introduce _ ==> _ with _. begin
+          assert (sem_typing g' body t2);
+          eliminate forall b (s:gsub g' b). gsub_only_values s ==> (gsubst s body) ⋮ t2 with false (gsub_extend s t1 v);
+          assert (gsubst (gsub_extend s t1 v) body ⋮ t2);
+          lem_substitution s t1 v body;
+          assert (subst_beta v body' ⋮ t2)
+        end
+      end;
+      assert (gsubst s (ELam body) ∈ TArr t1 t2);
+      lem_value_is_typed_exp (gsubst s (ELam body)) (TArr t1 t2)
+    end
 
 let typing_rule_app g (e1:exp) (e2:exp) (t1:typ) (t2:typ) : Lemma
   (requires sem_typing g e1 (TArr t1 t2) /\ sem_typing g e2 t1)
@@ -125,20 +104,21 @@ let typing_rule_app g (e1:exp) (e2:exp) (t1:typ) (t2:typ) : Lemma
   assert (fv_in_env g e1);
   assert (fv_in_env g e2);
   assume (fv_in_env g (EApp e1 e2)); (** should be proveable **)
-  introduce forall b (s:gsub g b). gsubst s (EApp e1 e2) ⋮ t2 with begin
-    introduce forall e'. steps (gsubst s (EApp e1 e2)) e' /\ irred e' ==> e' ∈ t2 with begin
-      introduce _ ==> e' ∈ t2 with h. begin
-        let steps_e_e' : squash (steps (EApp (gsubst s e1) (gsubst s e2)) e') = () in
-        FStar.Squash.map_squash #_ #(squash (e' ∈ t2)) steps_e_e' (fun steps_e_e' ->
-          let (e11, e2') = destruct_steps_eapp (gsubst s e1) (gsubst s e2) e' steps_e_e' in
-          assert (ELam e11 ∈ TArr t1 t2);
-          assert (e2' ∈ t1);
-          assert (subst_beta e2' e11 ⋮ t2);
-          assert (e' ∈ t2)
-        )
+  introduce forall b (s:gsub g b). gsub_only_values s ==> gsubst s (EApp e1 e2) ⋮ t2 with
+    introduce gsub_only_values s ==> gsubst s (EApp e1 e2) ⋮ t2 with _. begin
+      introduce forall e'. steps (gsubst s (EApp e1 e2)) e' /\ irred e' ==> e' ∈ t2 with begin
+        introduce _ ==> e' ∈ t2 with h. begin
+          let steps_e_e' : squash (steps (EApp (gsubst s e1) (gsubst s e2)) e') = () in
+          FStar.Squash.map_squash #_ #(squash (e' ∈ t2)) steps_e_e' (fun steps_e_e' ->
+            let (e11, e2') = destruct_steps_eapp (gsubst s e1) (gsubst s e2) e' steps_e_e' in
+            assert (ELam e11 ∈ TArr t1 t2);
+            assert (e2' ∈ t1);
+            assert (subst_beta e2' e11 ⋮ t2);
+            assert (e' ∈ t2)
+          )
+        end
       end
     end
-  end
 
 let typing_rule_if g (e1:exp) (e2:exp) (e3:exp) (t:typ) : Lemma
   (requires sem_typing g e1 TBool /\ sem_typing g e2 t /\ sem_typing g e3 t)
@@ -147,15 +127,16 @@ let typing_rule_if g (e1:exp) (e2:exp) (e3:exp) (t:typ) : Lemma
   assert (fv_in_env g e2);
   assert (fv_in_env g e3);
   assume (fv_in_env g (EIf e1 e2 e3)); (** should be proveable **)
-  introduce forall b (s:gsub g b). gsubst s (EIf e1 e2 e3) ⋮ t with begin
-    introduce forall e'. steps (gsubst s (EIf e1 e2 e3)) e' /\ irred e' ==> e' ∈ t with begin
-      introduce _ ==> e' ∈ t with h. begin
-        let steps_e_e' : squash (steps (EIf (gsubst s e1) (gsubst s e2) (gsubst s e3)) e') = () in
-        FStar.Squash.map_squash #_ #(squash (e' ∈ t)) steps_e_e' (fun steps_e_e' ->
-          let e1' = destruct_steps_eif (gsubst s e1) (gsubst s e2) (gsubst s e3) e' steps_e_e' in
-          assert (e1' ∈ TBool);
-          assert (e' ∈ t)
-        )
+  introduce forall b (s:gsub g b). gsub_only_values s ==> gsubst s (EIf e1 e2 e3) ⋮ t with
+    introduce gsub_only_values s ==> gsubst s (EIf e1 e2 e3) ⋮ t with _. begin
+      introduce forall e'. steps (gsubst s (EIf e1 e2 e3)) e' /\ irred e' ==> e' ∈ t with begin
+        introduce _ ==> e' ∈ t with h. begin
+          let steps_e_e' : squash (steps (EIf (gsubst s e1) (gsubst s e2) (gsubst s e3)) e') = () in
+          FStar.Squash.map_squash #_ #(squash (e' ∈ t)) steps_e_e' (fun steps_e_e' ->
+            let e1' = destruct_steps_eif (gsubst s e1) (gsubst s e2) (gsubst s e3) e' steps_e_e' in
+            assert (e1' ∈ TBool);
+            assert (e' ∈ t)
+          )
+        end
       end
     end
-  end
