rupicola/SyntacticTypes.fst
@@ -22,7 +22,7 @@ let rec elab_typ (t:typ) : Type0 =
   | TBool -> bool
   | TArr t1 t2 -> (elab_typ t1 -> elab_typ t2)
 
-(** Common definition of typing environment **)
+(** Typing environment **)
 type env = var -> option typ
 
 let empty : env = fun _ -> None
@@ -41,3 +41,29 @@ let lem_no_fv_is_closed (e:exp) : Lemma
   (ensures is_closed e)
   [SMTPat (is_closed e)] =
   ()
+
+(** STLC Evaluation Environment : variable -> value **)
+let gsub (g:env) (b:bool{b ==> (forall x. None? (g x))}) = (** CA: this b is polluting **)
+  s:(sub b){forall x. Some? (g x) ==> is_value (s x)}
+
+let gsub_empty : gsub empty true =
+  (fun v -> EVar v)
+
+let gsub_extend (#g:env) #b (s:gsub g b) (t:typ) (v:value) : gsub (extend t g) false =
+  let f = fun (y:var) -> if y = 0 then v else s (y-1) in
+  introduce exists (x:var). ~(EVar? (f x)) with 0 and ();
+  f
+
+let gsubst (#g:env) #b (s:gsub g b) (e:exp{fv_in_env g e}) : closed_exp =
+  lem_subst_freevars_closes_exp s e 0;
+  subst s e
+
+let lem_substitution #g #b (s:gsub g b) (t:typ) (v:value) (e:exp)
+  : Lemma (
+    (subst (sub_beta v) (subst (sub_elam s) e)) == (subst (gsub_extend s t v) e))
+  = admit () (** common lemma **)
+
+let lem_gsubst_empty_identity (e:closed_exp) :
+  Lemma (gsubst gsub_empty e == e)
+  [SMTPat (gsubst gsub_empty e)] =
+  admit ()
